src/coq/Handlers/MemoryModules/Within.v
@@ -99,3 +99,59 @@ Section Laws.
       within_ret_refl : forall {A} (x : A), ret x ∈ ret x;
     }.
 End Laws.
+
+Definition transitive_within {Pre Post} {M1 M2 M3} `{EQM2 : Eq1 M2} `{EQM3 : Eq1 M3} `{WM1M2 : @Within M2 EQM2 M1 Pre Post} `{WM2M3 : @Within M3 EQM3 M2 Pre Post}
+  {A} (m3 : M3 A) (pre : Pre) (m1 : M1 A) (post : Post) : Prop :=
+  exists (m2 : M2 A),
+    (m1 {{pre}} ∈ {{post}} m2) /\
+      (m2 {{pre}} ∈ {{post}} m3).
+
+Definition transitive_within_eq1_Proper {Pre Post} {M1 M2 M3} `{EQM2 : Eq1 M2} `{EQM3 : Eq1 M3} `{WM1M2 : @Within M2 EQM2 M1 Pre Post} `{WM2M3 : @Within M3 EQM3 M2 Pre Post} {A} :
+  Proper (eq1 ==> eq ==> eq ==> eq ==> iff) (transitive_within (A:=A)).
+Proof.
+  unfold Proper, respectful.
+  intros x y H x0 y0 H0 x1 y1 H1 x2 y2 H2.
+  subst.
+  unfold transitive_within.
+  split; intros [m2 [INM2 INM3]].
+  - rewrite H in INM3.
+    exists m2; split; auto.
+  - rewrite <- H in INM3.
+    exists m2; split; auto.
+Defined.
+
+#[global] Instance Transitive_Within {Pre Post} {M1 M2 M3} `{EQM2 : Eq1 M2} `{EQM3 : Eq1 M3} `{WM1M2 : @Within M2 EQM2 M1 Pre Post} `{WM2M3 : @Within M3 EQM3 M2 Pre Post} : @Within M3 EQM3 M1 Pre Post.
+Proof.
+  esplit.
+  intros A.
+  unfold Proper, respectful.
+  intros x y H x0 y0 H0 x1 y1 H1 x2 y2 H2.
+  eapply transitive_within_eq1_Proper; eauto.
+Defined.
+
+Definition reflexive_within {Pre Post} {M} `{EQM : Eq1 M}
+  {A} (m : M A) (pre : Pre) (m' : M A) (post : Post) : Prop :=
+  m ≈ m'.
+
+Definition reflexive_within_eq1_Proper {Pre Post} {M} `{MM : Monad M} `{EQM : Eq1 M} `{EQV : @Eq1Equivalence M MM EQM} {A} :
+  Proper (eq1 ==> eq ==> eq ==> eq ==> iff) (reflexive_within (Pre:=Pre) (Post:=Post) (A:=A)).
+Proof.
+  unfold Proper, respectful.
+  intros x y H x0 y0 H0 x1 y1 H1 x2 y2 H2.
+  subst.
+  unfold reflexive_within.
+  split; intros EQ.
+  - rewrite <- H.
+    auto.
+  - rewrite H.
+    auto.
+Defined.
+
+#[global] Instance Reflexive_Within {Pre Post} {M} `{MM : Monad M} `{EQM : Eq1 M} `{EQV : @Eq1Equivalence M MM EQM} : @Within M EQM M Pre Post.
+Proof.
+  esplit.
+  intros A.
+  unfold Proper, respectful.
+  intros x y H x0 y0 H0 x1 y1 H1 x2 y2 H2.
+  eapply reflexive_within_eq1_Proper; eauto.
+Defined.
